examples/QueryStructure/Messages.v
@@ -65,122 +65,12 @@ Definition MessagesSpec : ADT MessagesSig :=
 }.
 
 Definition SharpenedMessages :
-  Sharpened MessagesSpec.
+  MostlySharpened MessagesSpec.
 Proof.
 
-  Unset Ltac Debug.
-  unfold MessagesSpec.
-
-  start honing QueryStructure.
-
-  GenerateIndexesForAll matchInclusionClause ltac:(fun l => make simple indexes using l).
-
-
-    hone method "AddMessage".
-  {
-    Implement_Insert_Checks.
-    Focused_refine_Query.
-    {
-      (* Step 1: Implement [In] by enumeration. *)
-      implement_In;
-      (* Step 2: Convert where clauses into compositions of filters. *)
-      repeat convert_Where_to_filter.
-      (* Step 3: Do some simplication.*)
-    repeat setoid_rewrite <- filter_and;
-    try setoid_rewrite andb_true_r.
-    (* Step 4: Move filters to the outermost [Join_Comp_Lists] to which *)
-    (* they can be applied. *)
-    repeat setoid_rewrite Join_Filtered_Comp_Lists_id;
-    distribute_filters_to_joins.
-    (* Step 5: Convert filter function on topmost [Join_Filtered_Comp_Lists] to an
-               equivalent search term matching function.  *)
-    implement_filters_with_find
-      ltac:(find_simple_search_term
-              InclusionIndexUse createLastInclusionTerm createEarlyInclusionTerm)
-             ltac:(find_simple_search_term_dep
-                     InclusionIndexUse_dep createLastInclusionTerm_dep createEarlyInclusionTerm_dep).
-  |
-  ].
-
-InclusionIndexUse createLastInclusionTerm createEarlyInclusionTerm
-      InclusionIndexUse_dep createLastInclusionTerm_dep createEarlyInclusionTerm_dep.
-
-    implement_Query.
-    simpl; simplify with monad laws.
-    setoid_rewrite refineEquiv_swap_bind.
-    implement_Insert_branches.
-
-    cleanup_Count.
-    finish honing.
-  }
-  hone method "RelevantMessages".
-  {
-    implement_Query InclusionIndexUse createLastInclusionTerm createEarlyInclusionTerm
-      InclusionIndexUse_dep createLastInclusionTerm_dep createEarlyInclusionTerm_dep.
-    (* Do some more simplication using the monad laws. *)
-    simpl; simplify with monad laws.
-    (* Satisfied with the query, we now implement the new data
-       representation (in this case, it is unchanged).
-     *)
-    simpl; commit.
-    repeat setoid_rewrite filter_true;
-      repeat setoid_rewrite app_nil_r;
-      repeat setoid_rewrite map_length.
-    finish honing.
-  }
-
-  hone method "ContactMessages".
-  {
-    implement_Query InclusionIndexUse createLastInclusionTerm createEarlyInclusionTerm
-      InclusionIndexUse_dep createLastInclusionTerm_dep createEarlyInclusionTerm_dep.
-    simpl; simplify with monad laws.
-    simpl; commit.
-    repeat setoid_rewrite filter_true;
-      repeat setoid_rewrite app_nil_r;
-      repeat setoid_rewrite map_length.
-    finish honing.
-  }
-
-  hone constructor "Init".
-  {
-    simplify with monad laws.
-    rewrite refine_QSEmptySpec_Initialize_IndexedQueryStructure.
-    simpl.
-    finish honing.
-  }
-
-  hone method "AddMessage".
-  {
-    Implement_Insert_Checks.
-
-    implement_Query.
-    simpl; simplify with monad laws.
-    setoid_rewrite refineEquiv_swap_bind.
-    implement_Insert_branches.
-
-    cleanup_Count.
-    finish honing.
-  }
-
-  hone method "AddContact".
-  {
-    Implement_Insert_Checks.
-
-    implement_Query.
-    simpl; simplify with monad laws.
-    setoid_rewrite refineEquiv_swap_bind.
-    implement_Insert_branches.
-
-    cleanup_Count.
-    finish honing.
-  }
+  partial_master_plan InclusionIndexTactics.
 
   FullySharpenQueryStructure MessagesSchema Index.
-
-  implement_bag_methods.
-  implement_bag_methods.
-  implement_bag_methods.
-  implement_bag_methods.
 
 Time Defined.
 
